Finished the typing rules for terms and proof terms

src/Logic.v
@@ -4,6 +4,7 @@
 *)
 
 Require Import Arith.
+Require Import ZArith.
 Require Import List.
 Require Import Utils.
 Import ListNotations.
@@ -22,24 +23,30 @@ Set Implicit Arguments.
 
 (** ** The Syntax *)
 
+(** Constants *)
+Definition const := positive.
+
 (** Types *)
 Inductive ty : Type :=
 | prop
-| tcst
+| bty 
 | arr : ty -> ty -> ty.
 
 (** Terms *)
 Inductive term: Type :=
-| cst
+| cst  : const -> term
 | fvar : nat -> term
 | bvar : nat -> term
 | abs  : ty -> term -> term
 | app  : term -> term -> term
-| eq   : term -> term -> term.
+| teq   : term -> term -> term.
+
+Notation "t1 == t2" := (teq t1 t2) (at level 60) : stlcd_scope.
+
+Local Open Scope stlcd_scope.
 
 (** Proof terms *)
 Inductive pterm: Type :=
-| pcst
 | refl: term -> pterm
 | trans: pterm -> pterm -> pterm
 | symm : pterm -> pterm
@@ -63,21 +70,22 @@ Definition sub := list term.
 (** Freshening of terms *)
 Fixpoint fresh_tm (t:term) (bn fn: nat) : term :=
   match t with
-  | cst => cst
+  | cst _ => t
   | fvar _ => t
   | bvar i => if beq_nat i bn then fvar fn else t
   | abs ty t => 
     abs ty (fresh_tm t (S bn) fn)
   | app t1 t2 =>
     app (fresh_tm t1 bn fn) (fresh_tm t2 bn fn)
-  | eq t1 t2 =>
-    eq (fresh_tm t1 bn fn) (fresh_tm t2 bn fn)
+  | t1 == t2 =>
+    (fresh_tm t1 bn fn) == (fresh_tm t2 bn fn)
   end.
+
+Definition fresh_tm_0 t fn := fresh_tm t 0 fn.
 
 (** Freshening of proof terms *)
 Fixpoint fresh_ptm (pt:pterm) (bn fn: nat) : pterm :=
   match pt with
-  | pcst => pcst
   | refl t => refl (fresh_tm t bn fn)
   | trans pt1 pt2 => 
     trans (fresh_ptm pt1 bn fn) (fresh_ptm pt2 bn fn)
@@ -99,24 +107,28 @@ Fixpoint fresh_ptm (pt:pterm) (bn fn: nat) : pterm :=
     conv (fresh_ptm pt1 bn fn) (fresh_ptm pt2 bn fn)
 end.
 
+Definition fresh_ptm_0 t fn := fresh_ptm t 0 fn.
+
+
 (** Binding of terms *)
 Fixpoint bind_tm (t:term) (bn fn: nat) : term :=
   match t with
-  | cst => cst
+  | cst _ => t
   | fvar i => if beq_nat i fn then bvar bn else t
   | bvar i => t 
   | abs ty t => 
     abs ty (bind_tm t (S bn) fn)
   | app t1 t2 =>
     app (bind_tm t1 bn fn) (bind_tm t2 bn fn)
-  | eq t1 t2 =>
-    eq (bind_tm t1 bn fn) (bind_tm t2 bn fn)
+  | t1 == t2 =>
+    (bind_tm t1 bn fn) == (bind_tm t2 bn fn)
   end.
   
+Definition bind_tm_0 t fn := bind_tm t 0 fn.
+
 (** Binding of proof terms *)
 Fixpoint bind_ptm (pt:pterm) (bn fn: nat) : pterm :=
   match pt with
-  | pcst => pcst
   | refl t => refl (fresh_tm t bn fn)
   | trans pt1 pt2 => 
     trans (bind_ptm pt1 bn fn) (bind_ptm pt2 bn fn)
@@ -138,35 +150,54 @@ Fixpoint bind_ptm (pt:pterm) (bn fn: nat) : pterm :=
     conv (bind_ptm pt1 bn fn) (bind_ptm pt2 bn fn)
 end.
 
+Definition bind_ptm_0 t fn := bind_ptm t 0 fn.
+
 
 (** ** Operations on substitutions *)
 
-(** Access the i-th element of a substitution *)
-Module ALT_SUB_INDEX.
-Program Fixpoint index_sub (s:sub) (i: {n:nat | n < length s}) : term :=
-  match s with
-  | [] => False_rec _ _
-  | t :: s' => 
-    match (proj1_sig i) with
-    | O => t
-    | S i' => index_sub s' (exist _ i' _)
-    end
+(** Generate identity substitutions *)
+Fixpoint idsub_acc (acc:sub) (n:nat) : sub :=
+  match n with
+  | O => acc
+  | S n' => idsub_acc (fvar (length acc)::acc) n'
   end.
-Next Obligation.
-  simpl in H. eapply Nat.nlt_0_r; eauto.
-Defined.
-Next Obligation.
-  simpl in H. apply lt_S_n. auto.
-Defined.
-End ALT_SUB_INDEX.
+
+Compute (idsub_acc [] 11).
+
+Definition idsub (n:nat) : sub :=
+  idsub_acc [] n.
+
+(** Access the i-th element of a substitution *)
+(* Module ALT_SUB_INDEX. *)
+(* Program Fixpoint index_sub (s:sub) (i: {n:nat | n < length s}) : term := *)
+(*   match s with *)
+(*   | [] => False_rec _ _ *)
+(*   | t :: s' =>  *)
+(*     match (proj1_sig i) with *)
+(*     | O => t *)
+(*     | S i' => index_sub s' (exist _ i' _) *)
+(*     end *)
+(*   end. *)
+(* Next Obligation. *)
+(*   simpl in H. eapply Nat.nlt_0_r; eauto. *)
+(* Defined. *)
+(* Next Obligation. *)
+(*   simpl in H. apply lt_S_n. auto. *)
+(* Defined. *)
+(* End ALT_SUB_INDEX. *)
 
 Definition index_sub (s:sub) (i:nat) : option term :=
-  nth_error s i.
+  if Nat.leb i (length s -1) then 
+    nth_error s (length s - 1 - i)
+  else
+    None.
+
+Compute (index_sub (idsub_acc [] 11) 10).
 
 (** Application of substitution to terms *)
 Fixpoint app_sub_tm (t:term) (s:sub) : option term :=
   match t with
-  | cst => Some cst
+  | cst _ => Some t
   | fvar i => index_sub s i
   | bvar _ => Some t
   | abs ty t1 =>
@@ -176,16 +207,15 @@ Fixpoint app_sub_tm (t:term) (s:sub) : option term :=
     do t1' <- app_sub_tm t1 s;
     do t2' <- app_sub_tm t2 s;
     Some (app t1' t2')
-  | eq t1 t2 =>
+  | t1 == t2 =>
     do t1' <- app_sub_tm t1 s;
     do t2' <- app_sub_tm t2 s;
-    Some (eq t1' t2')
+    Some (t1' == t2')
   end.
 
 (** Application of substitution to proof terms *)
 Fixpoint app_sub_ptm (pt:pterm) (s:sub) : option pterm :=
   match pt with
-  | pcst => Some pcst
   | refl t => 
     do t' <- app_sub_tm t s;
     Some (refl t')
@@ -220,3 +250,79 @@ Fixpoint app_sub_ptm (pt:pterm) (s:sub) : option pterm :=
     do pt2' <- app_sub_ptm pt2 s;
     Some (conv pt1' pt2')
 end.
+
+(** ** Operations on typing contexts *)
+Definition index_ctx (ctx:tyctx) (i:nat) : option ty :=
+  if Nat.leb i (length ctx -1) then 
+    nth_error ctx (length ctx - 1 - i)
+  else
+    None.
+
+
+(** ** Typing rules *)
+
+(** Signatures *)
+Definition sign := const -> ty.
+
+(** Typing rules for terms *)
+Inductive tm_of: sign -> tyctx -> term -> ty -> Prop :=
+| tm_of_cst : forall sgn ctx c ty, sgn c = ty -> tm_of sgn ctx (cst c) ty
+| tm_of_fvar : forall sgn ctx i ty,
+    index_ctx ctx i = Some ty ->
+    tm_of sgn ctx (fvar i) ty
+| tm_of_abs : forall sgn ctx ty1 ty2 t n,
+    length ctx = n ->
+    tm_of sgn (ty1::ctx) (fresh_tm_0 t n) ty2 ->
+    tm_of sgn ctx (abs ty1 t) (arr ty1 ty2)
+| tm_of_app : forall sgn ctx t1 t2 ty1 ty2,
+    tm_of sgn ctx t1 (arr ty1 ty2) -> 
+    tm_of sgn ctx t2 ty1 -> 
+    tm_of sgn ctx (app t1 t2) ty2
+| tm_of_eq : forall sgn ctx t1 t2 ty,
+    tm_of sgn ctx t1 ty -> 
+    tm_of sgn ctx t2 ty -> 
+    tm_of sgn ctx (t1 == t2) prop.
+
+
+(** Typing rules for proof terms *)
+Inductive ptm_of: sign -> tyctx -> pterm -> term -> Prop :=
+| ptm_of_refl: forall sgn ctx t ty,
+    tm_of sgn ctx t ty ->
+    ptm_of sgn ctx (refl t) (t == t)
+| ptm_of_trans: forall sgn ctx pt1 pt2 t1 t2 t3,
+    ptm_of sgn ctx pt1 (t1 == t2) ->
+    ptm_of sgn ctx pt2 (t2 == t3) ->
+    ptm_of sgn ctx (trans pt1 pt2) (t1 == t3)
+| ptm_of_symm: forall sgn ctx pt t1 t2,
+    ptm_of sgn ctx pt (t2 == t1) ->
+    ptm_of sgn ctx (symm pt) (t1 == t2)
+| ptm_of_congAbs: forall sgn ctx ty pt t1 t2 n,
+    length ctx = n ->
+    ptm_of sgn (ty::ctx) (fresh_ptm_0 pt n) (t1 == t2) -> 
+    ptm_of sgn ctx (congAbs ty pt) 
+           (abs ty (bind_tm_0 t1 (length ctx)) == abs ty (bind_tm_0 t2 n))
+| ptm_of_congAppL: forall sgn ctx pt t1 t1' t2,
+    ptm_of sgn ctx pt (t1 == t1') ->
+    ptm_of sgn ctx (congAppL pt) (app t1 t2 == app t1' t2)
+| ptm_of_congAppR: forall sgn ctx pt t1 t2 t2',
+    ptm_of sgn ctx pt (t2 == t2') ->
+    ptm_of sgn ctx (congAppR pt) (app t1 t2 == app t1 t2')
+| ptm_of_congEqL: forall sgn ctx pt t1 t1' t2,
+    ptm_of sgn ctx pt (t1 == t1') ->
+    ptm_of sgn ctx (congEqL pt) ((t1 == t2) == (t1' == t2))
+| ptm_of_congEqR: forall sgn ctx pt t1 t2 t2',
+    ptm_of sgn ctx pt (t2 == t2') ->
+    ptm_of sgn ctx (congEqR pt) ((t1 == t2) == (t1 == t2'))
+| ptm_of_beta: forall sgn ctx t1 t2 t3 n ty1 ty2,
+    length ctx = n ->
+    tm_of sgn ctx (abs ty1 t1) (arr ty1 ty2) ->
+    tm_of sgn ctx t2 ty1 ->
+    app_sub_tm (fresh_tm_0 t1 n) (t2::(idsub n)) = Some t3 ->
+    ptm_of sgn ctx (beta ty1 t1 t2) 
+           (app (abs ty1 t1) t2 == t3)
+| ptm_of_conv: forall sgn ctx pt1 pt2 t1 t2,
+    ptm_of sgn ctx pt1 t1 ->
+    ptm_of sgn ctx pt2 (t1 == t2) ->
+    ptm_of sgn ctx (conv pt1 pt2) t2.
+
+
